P256.MM

code/ecdsap256/Hacl.Impl.P256.MontgomeryMultiplication.fst
@@ -102,48 +102,43 @@ let montgomery_multiplication_round_twice t result =
   pop_frame()
 
 
-val montgomery_multiplication_buffer_by_one: a: felem P256 -> result: felem P256 -> Stack unit
-  (requires (fun h -> live h a /\ as_nat P256 h a < prime256 /\ live h result)) 
-  (ensures (fun h0 _ h1 -> 
-    modifies (loc result) h0 h1 /\ 
-    as_nat P256 h1 result  = (as_nat P256 h0 a * modp_inv2_prime (pow2 256) prime256) % prime256 /\
-    as_nat P256 h1 result = fromDomain_ #P256 (as_nat P256 h0 a))
-  )
 
-
-let montgomery_multiplication_buffer_by_one a result = 
-  assert_norm (prime256 > 3);
-  push_frame();
-    let t = create (size 8) (u64 0) in 
-      let t_low = sub t (size 0) (size 4) in 
-      let t_high = sub t (size 4) (size 4) in 
-    let round2 = create (size 8) (u64 0) in 
-    let round4 = create (size 8) (u64 0) in  
-      let h0 = ST.get() in 
-    copy t_low a; 
-      let h1 = ST.get() in 
-      assert(wide_as_nat P256 h0 t = as_nat P256 h0 t_low + as_nat P256 h0 t_high * pow2 256);
-      assert_norm (prime256 < prime256 * prime256);
-    montgomery_multiplication_round_twice t round2;
-      let h2 = ST.get() in 
-    montgomery_multiplication_round_twice round2 round4; 
-      lemma_montgomery_mod_inverse_addition2 (wide_as_nat P256 h1 t);
-      lemma_mod_mul_distr_l (wide_as_nat P256 h2 round2) (modp_inv2_prime (pow2 128) prime256) prime256;
-      lemma_mod_mul_distr_l (wide_as_nat P256 h1 t * modp_inv2_prime (pow2 128) prime256) (modp_inv2_prime (pow2 128) prime256) prime256;
-	mul_lemma_2 (wide_as_nat P256 h1 t % pow2 64) (pow2 64 - 1) prime256;
-	mul_lemma_2 (let round = (wide_as_nat P256 h1 t + prime256 * (wide_as_nat P256 h1 t % pow2 64)) / pow2 64 in round % pow2 64) (pow2 64 - 1) prime256;
-	mul_lemma_2 (
-	  let round = (wide_as_nat P256 h1 t + prime256 * (wide_as_nat P256 h1 t % pow2 64)) / pow2 64 in  
-	  let round2 = (round + prime256 * (round % pow2 64)) / pow2 64 in 
-	  round2 % pow2 64) (pow2 64 - 1) prime256;
-	mul_lemma_2 (	
-	  let round = (wide_as_nat P256 h1 t + prime256 * (wide_as_nat P256 h1 t % pow2 64)) / pow2 64 in  
-	  let round2 = (round + prime256 * (round % pow2 64)) / pow2 64 in 
-	  let round3 = (round2 + prime256 * (round2 % pow2 64)) / pow2 64 in   
-	  round3 % pow2 64) (pow2 64 - 1) prime256;
-    reduction_prime256_2prime256_8_with_carry_impl round4 result;
-    lemmaFromDomain #P256 (as_nat P256 h0 a);
-  pop_frame()  
+let montgomery_multiplication_buffer_by_one #c a result = 
+  match c with 
+  |P384 -> ()
+  |P256 -> 
+    assert_norm (prime256 > 3);
+    push_frame();
+      let t = create (size 8) (u64 0) in 
+	let t_low = sub t (size 0) (size 4) in 
+	let t_high = sub t (size 4) (size 4) in 
+      let round2 = create (size 8) (u64 0) in 
+      let round4 = create (size 8) (u64 0) in  
+	let h0 = ST.get() in 
+      copy t_low a; 
+	let h1 = ST.get() in 
+	assert(wide_as_nat P256 h0 t = as_nat P256 h0 t_low + as_nat P256 h0 t_high * pow2 256);
+	assert_norm (prime256 < prime256 * prime256);
+      montgomery_multiplication_round_twice t round2;
+	let h2 = ST.get() in 
+      montgomery_multiplication_round_twice round2 round4; 
+	lemma_montgomery_mod_inverse_addition2 (wide_as_nat P256 h1 t);
+	lemma_mod_mul_distr_l (wide_as_nat P256 h2 round2) (modp_inv2_prime (pow2 128) prime256) prime256;
+	lemma_mod_mul_distr_l (wide_as_nat P256 h1 t * modp_inv2_prime (pow2 128) prime256) (modp_inv2_prime (pow2 128) prime256) prime256;
+	  mul_lemma_2 (wide_as_nat P256 h1 t % pow2 64) (pow2 64 - 1) prime256;
+	  mul_lemma_2 (let round = (wide_as_nat P256 h1 t + prime256 * (wide_as_nat P256 h1 t % pow2 64)) / pow2 64 in round % pow2 64) (pow2 64 - 1) prime256;
+	  mul_lemma_2 (
+	    let round = (wide_as_nat P256 h1 t + prime256 * (wide_as_nat P256 h1 t % pow2 64)) / pow2 64 in  
+	    let round2 = (round + prime256 * (round % pow2 64)) / pow2 64 in 
+	    round2 % pow2 64) (pow2 64 - 1) prime256;
+	  mul_lemma_2 (	
+	    let round = (wide_as_nat P256 h1 t + prime256 * (wide_as_nat P256 h1 t % pow2 64)) / pow2 64 in  
+	    let round2 = (round + prime256 * (round % pow2 64)) / pow2 64 in 
+	    let round3 = (round2 + prime256 * (round2 % pow2 64)) / pow2 64 in   
+	    round3 % pow2 64) (pow2 64 - 1) prime256;
+      reduction_prime_2prime_with_carry  round4 result;
+      lemmaFromDomain #P256 (as_nat P256 h0 a);
+    pop_frame()  
 
 
 val montgomery_multiplication_buffer_p256: a: felem P256 -> b: felem P256 -> result: felem P256 ->  Stack unit
@@ -189,7 +184,7 @@ let montgomery_multiplication_buffer_p256 a b result =
 	let round3 = (round2 + prime256 * (round2 % pow2 64)) / pow2 64 in 
 	round3 % pow2 64) (pow2 64) prime256;  
       assert_norm((prime256 * pow2 64 + (prime256 * pow2 64 + (prime256 * pow2 64 + ((pow2 64 - 1) * prime256 + prime256 * prime256) / pow2 64) / pow2 64)/ pow2 64) / pow2 64 < 2 * prime256);
-  reduction_prime256_2prime256_8_with_carry_impl round4 result; 
+  reduction_prime_2prime_with_carry round4 result; 
   lemmaFromDomainToDomain #P256 (as_nat P256 h0 a);
   lemmaFromDomainToDomain #P256 (as_nat P256 h0 b);
   multiplicationInDomainNat #P256 #(fromDomain_ #P256 (as_nat P256 h0 a)) #(fromDomain_ #P256 (as_nat P256 h0 b))  (as_nat P256 h0 a) (as_nat P256 h0 b);
@@ -197,15 +192,6 @@ let montgomery_multiplication_buffer_p256 a b result =
   pop_frame()  
 
 
-val montgomery_multiplication_buffer: #c: curve -> a: felem c -> b: felem c -> result: felem c ->  Stack unit
-  (requires (fun h -> live h a /\ as_nat c h a < getPrime c /\ live h b /\ live h result /\ as_nat c h b < getPrime c)) 
-  (ensures (fun h0 _ h1 -> 
-    modifies (loc result) h0 h1 /\  
-    as_nat c h1 result < getPrime c /\
-    as_nat c h1 result = (as_nat c h0 a * as_nat c h0 b * modp_inv2_prime (pow2 (getPower c)) (getPrime c)) % getPrime c /\
-    as_nat c h1 result = toDomain_ #c (fromDomain_ #c (as_nat c h0 a) * fromDomain_ #c (as_nat c h0 b) % getPrime c) /\
-    as_nat c h1 result = toDomain_ #c (fromDomain_ #c (as_nat c h0 a) * fromDomain_ #c (as_nat c h0 b)))
-  )
 
 
 let montgomery_multiplication_buffer #c a b result = 
@@ -214,18 +200,6 @@ let montgomery_multiplication_buffer #c a b result =
   |P384 -> admit()
 
 
-val montgomery_square_buffer: #c: curve -> a: felem c -> result: felem c ->  Stack unit
-  (requires (fun h -> live h a /\ as_nat c h a < (getPrime c) /\ live h result)) 
-  (ensures (fun h0 _ h1 -> 
-    (
-      let prime = getPrime c in 
-      modifies (loc result) h0 h1 /\  
-      as_nat c h1 result < prime /\ 
-      as_nat c h1 result = (as_nat c h0 a * as_nat c h0 a * modp_inv2_prime (getPower c) prime) % prime /\
-      as_nat c h1 result = toDomain_ #c (fromDomain_ #c (as_nat c h0 a) * fromDomain_ #c (as_nat c h0 a) % prime) /\
-      as_nat c h1 result = toDomain_ #c (fromDomain_ #c (as_nat c h0 a) * fromDomain_ #c (as_nat c h0 a)))
-    )
-  )
 
 
 val montgomery_square_buffer_p256: a: felem P256 -> result: felem P256 -> Stack unit
@@ -252,7 +226,7 @@ let montgomery_square_buffer_p256 a result =
     let round2 = create (size 8) (u64 0) in 
     let round4 = create (size 8) (u64 0) in  
       let h0 = ST.get() in 
-    sq a t;  
+    square_p256 a t;  
       let h1 = ST.get() in 
       mul_lemma_ (as_nat P256 h0 a) (as_nat P256 h0 a) prime256;
     montgomery_multiplication_round_twice t round2;
@@ -274,7 +248,7 @@ let montgomery_square_buffer_p256 a result =
      let round3 = (round2 + prime256 * (round2 % pow2 64)) / pow2 64 in round3 % pow2 64) (pow2 64) prime256;  
       assert_norm((prime256 * pow2 64 + (prime256 * pow2 64 + (prime256 * pow2 64 + ((pow2 64 - 1) * prime256 + prime256 * prime256) / pow2 64) / pow2 64)/ pow2 64) / pow2 64 < 2 * prime256);
   
-   reduction_prime256_2prime256_8_with_carry_impl round4 result; 
+   reduction_prime_2prime_with_carry round4 result; 
    lemmaFromDomainToDomain #P256 (as_nat P256 h0 a);
    multiplicationInDomainNat #P256 #(fromDomain_ #P256 (as_nat P256 h0 a)) #(fromDomain_ #P256 (as_nat P256 h0 a))  (as_nat P256 h0 a) (as_nat P256 h0 a);
    inDomain_mod_is_not_mod #P256 (fromDomain_ #P256 (as_nat P256 h0 a) * fromDomain_ #P256 (as_nat P256 h0 a));
@@ -461,52 +435,49 @@ val lemma_mul_nat: a: nat -> b: nat -> Lemma (a * b >= 0)
 let lemma_mul_nat a b = ()
 
 
-val exponent: #c: curve ->  a: felem P256 -> result: felem P256 -> tempBuffer: lbuffer uint64 (size 20) ->  Stack unit
-  (requires fun h -> live h a /\ live h tempBuffer /\ live h result /\ disjoint tempBuffer result /\ 
-  disjoint a tempBuffer /\ as_nat P256 h a < prime256)
-  (ensures fun h0 _ h1 -> modifies2 result tempBuffer h0 h1 /\
-    (let k = fromDomain_ #c (as_nat c h0 a) in 
-    as_nat P256 h1 result =  toDomain_ #c ((pow k (prime256-2)) % prime256)))
 
 
 #reset-options " --z3rlimit 200"
 let exponent #c a result tempBuffer = 
-  let h0 = ST.get () in 
-  let buffer_norm_1 = Lib.Buffer.sub  tempBuffer (size 0) (size 8) in 
-    let buffer_result1 = Lib.Buffer.sub tempBuffer (size 4) (size 4) in 
-  let buffer_result2 = Lib.Buffer.sub tempBuffer (size 8) (size 4) in 
-  let buffer_norm_3 = Lib.Buffer.sub tempBuffer (size 12) (size 8) in 
-    let buffer_result3 = Lib.Buffer.sub tempBuffer (size 16) (size 4) in 
- 
-  norm_part_one a buffer_norm_1;
-  norm_part_two a buffer_result2;
-  norm_part_three a buffer_norm_3;
+  match c with 
+  |P384 -> ()
+  |P256 -> 
+    let h0 = ST.get () in 
+    let buffer_norm_1 = Lib.Buffer.sub  tempBuffer (size 0) (size 8) in 
+      let buffer_result1 = Lib.Buffer.sub tempBuffer (size 4) (size 4) in 
+    let buffer_result2 = Lib.Buffer.sub tempBuffer (size 8) (size 4) in 
+    let buffer_norm_3 = Lib.Buffer.sub tempBuffer (size 12) (size 8) in 
+      let buffer_result3 = Lib.Buffer.sub tempBuffer (size 16) (size 4) in 
   
-    let h1 = ST.get() in 
-  montgomery_multiplication_buffer #c buffer_result1 buffer_result2 buffer_result1;
-    let h2 = ST.get() in 
-  montgomery_multiplication_buffer #c buffer_result1 buffer_result3 buffer_result1;
-    let h3 = ST.get() in 
-  montgomery_multiplication_buffer #c buffer_result1 a buffer_result1;
-    let h4 = ST.get() in 
-  copy result buffer_result1; 
-    let h5 = ST.get() in 
-  assert_norm ((pow2 32 - 1) * pow2 224 >= 0);
-  assert_norm (pow2 192 >= 0);
-  assert_norm ((pow2 94 - 1) * pow2 2 >= 0);
+    norm_part_one a buffer_norm_1;
+    norm_part_two a buffer_result2;
+    norm_part_three a buffer_norm_3;
+    
+      let h1 = ST.get() in 
+    montgomery_multiplication_buffer #c buffer_result1 buffer_result2 buffer_result1;
+      let h2 = ST.get() in 
+    montgomery_multiplication_buffer #c buffer_result1 buffer_result3 buffer_result1;
+      let h3 = ST.get() in 
+    montgomery_multiplication_buffer #c buffer_result1 a buffer_result1;
+      let h4 = ST.get() in 
+    copy result buffer_result1; 
+      let h5 = ST.get() in 
+    assert_norm ((pow2 32 - 1) * pow2 224 >= 0);
+    assert_norm (pow2 192 >= 0);
+    assert_norm ((pow2 94 - 1) * pow2 2 >= 0);
 
-  
-  let k = fromDomain_ #c (as_nat P256 h0 a) in 
-  let power1 = pow k ((pow2 32 - 1) * pow2 224) in 
-  let power2 = pow k (pow2 192) in 
-  let power3 = pow k ((pow2 94 - 1) * pow2 2) in 
-  let power4 = pow k 1 in 
+    
+    let k = fromDomain_ #c (as_nat P256 h0 a) in 
+    let power1 = pow k ((pow2 32 - 1) * pow2 224) in 
+    let power2 = pow k (pow2 192) in 
+    let power3 = pow k ((pow2 94 - 1) * pow2 2) in 
+    let power4 = pow k 1 in 
 
-  lemma_mul_nat power1 power2;
+    lemma_mul_nat power1 power2;
 
-  lemma_inDomainModulo power1 power2;
-  lemma_inDomainModulo (power1 * power2) power3;
-  inDomain_mod_is_not_mod #c (((power1 * power2 * power3) % prime256 * power4));
-  lemma_mod_mul_distr_l (power1 * power2 * power3) power4 prime256;
-  big_power k ((pow2 32 - 1) * pow2 224) (pow2 192) ((pow2 94 -1 ) * pow2 2) 1;
-  assert_norm(((pow2 32 - 1) * pow2 224 + pow2 192 + (pow2 94 -1 ) * pow2 2 + 1) = prime256 - 2)
+    lemma_inDomainModulo power1 power2;
+    lemma_inDomainModulo (power1 * power2) power3;
+    inDomain_mod_is_not_mod #c (((power1 * power2 * power3) % prime256 * power4));
+    lemma_mod_mul_distr_l (power1 * power2 * power3) power4 prime256;
+    big_power k ((pow2 32 - 1) * pow2 224) (pow2 192) ((pow2 94 -1 ) * pow2 2) 1;
+    assert_norm(((pow2 32 - 1) * pow2 224 + pow2 192 + (pow2 94 -1 ) * pow2 2 + 1) = prime256 - 2)
