code/ecdsap256/Hacl.Impl.P256.LowLevel.PrimeSpecific.fst
@@ -21,12 +21,6 @@ open Lib.IntTypes.Intrinsics
 #reset-options " --z3rlimit 300"
 
 
-inline_for_extraction
-let prime256_buffer: x: glbuffer uint64 4ul {witnessed #uint64 #(size 4) x (Lib.Sequence.of_list p256_prime_list) /\ recallable x /\ felem_seq_as_nat (Lib.Sequence.of_list (p256_prime_list)) == prime256} = 
-  assert_norm (felem_seq_as_nat (Lib.Sequence.of_list (p256_prime_list)) == prime256);
-  createL_global p256_prime_list
-
-
 inline_for_extraction noextract
 val reduction_prime256_2prime256_with_carry_impl: cin: uint64 -> x: felem P256 -> result: felem P256 ->
   Stack unit 
