code/ecdsap256/Hacl.Impl.P256.LowLevel.PrimeSpecific.fsti
@@ -13,6 +13,11 @@ open Hacl.Spec.P256.MontgomeryMultiplication
 open FStar.Mul
 
 
+inline_for_extraction
+let prime256_buffer: x: glbuffer uint64 4ul {witnessed #uint64 #(size 4) x (Lib.Sequence.of_list p256_prime_list) /\ recallable x /\ felem_seq_as_nat (Lib.Sequence.of_list (p256_prime_list)) == prime256} = 
+  assert_norm (felem_seq_as_nat (Lib.Sequence.of_list (p256_prime_list)) == prime256);
+  createL_global p256_prime_list
+
 val reduction_prime_2prime_with_carry: #c: curve -> x: widefelem c -> result: felem c -> 
   Stack unit 
     (requires fun h -> 
